case_study/RiscvPmp/BlockVer/Spec.v
@@ -586,6 +586,13 @@ Module RiscvPmpBlockVerifSpec <: Specification RiscvPmpBase RiscvPmpSignature Ri
        lemma_precondition    :=
         ((term_val ty_xlenbits RiscvPmpIrisInstance.write_addr) = (term_var "paddr" +ᵇ term_sext (term_val (ty.bvec 12) immm))) ∗
         (term_var "r") ↦ᵣ (term_var "w") ∗
+        (* mmio_read (map_wordwidth widthh) = term_val (ty_word) (term_truncate (map_wordwidth widthh * byte) (term_var "w")) ∗ *)
+        (* term_binop (bop.relop bop.neq) *)
+        (*   ((term_binop bop.bvand *)
+        (*       (term_var "w") *)
+        (*       (term_val ty_word (bv.of_N 48)))) *)
+        (*   (term_val ty_word (bv.of_N 48)) = term_val ty.bool true; *)
+ 
         (term_binop bop.bvand (term_var "w") (term_val ty_word (bv.of_N 1)) =  (term_val ty_word (bv.of_N 0)));
       lemma_postcondition   :=
         asn_mmio_checked_write (map_wordwidth widthh) (term_var "paddr" +ᵇ term_sext (term_val (ty.bvec 12) immm)) (term_truncate (map_wordwidth widthh * byte) (term_var "w")) ∗
